theories/contexts.v
@@ -532,6 +532,7 @@ Proof.
     | faddr
     | eaddr
     | addr
+    | addr
     | n ces es
     | n f es
     ]; simpl in *; try by (injection Hdecomp as <- <- <-; unfold valid_ccs).
@@ -563,6 +564,7 @@ Proof.
     |
     | faddr
     | eaddr
+    | addr
     | addr
     | n ces es
     | n f es
@@ -681,6 +683,7 @@ Proof.
       |
       | faddr
       | eaddr
+      | addr
       | addr
       | n ces es
       | n f es
